galois/network/network_local_abs.lean
@@ -3,22 +3,22 @@ For a given agent, we define a labeled transition system
 where everything else occuring on the network may be completely arbitrary
 -/
 import .action
+       galois.network.network_implementation
+       galois.temporal.LTS
 
 namespace network
 namespace loc
 
 def next_agent_state_from_dlabel {A} {a_next : act A} (la : dlabel a_next)
   : A
-  := la.cont_result.snd 
+  := la.cont_result.snd
 
-inductive sends_message_st (P : socket → message_t → Prop) : agent_label → Prop
-| mk : ∀ sock mess plabel ms, P sock mess
-     → (sock, mess) ∈ ms
-     → sends_message_st (agent_label.poll plabel ms)
+def sends_message_st (P : socket → message_t → Prop) (l : agent_label) : Prop
+  := l.messages.Exists (λ x, P x.fst x.snd)
 
-inductive sends_message_std (P : socket → message_t → Prop) {ag : agent}
+def sends_message_std (P : socket → message_t → Prop) {ag : agent}
   (a_next : act ag.state_type) (la : dlabel a_next) : Prop
-| mk : ∀ sock mess, (sock, mess) ∈ la.messages → sends_message_std
+  := la.messages.Exists (λ x, P x.fst x.snd)
 
 section
 parameters {ag : agent}
@@ -32,13 +32,8 @@ end
 instance sends_message_st_decidable (P : socket → message_t → Prop) 
   [decP : ∀ x y, decidable (P x y)] : decidable_pred (sends_message_st P)
 := begin
-intros x, induction x,
-have H := list.Exists_decidable (λ x : socket × message_t, P x.fst x.snd) a_1,
-induction H,
-{ apply decidable.is_false, intros contra, cases contra,
-  apply a_2, 
-  admit },
-{ admit }
+intros x, unfold sends_message_st,
+apply list.Exists_decidable,
 end
 
 end
@@ -46,4 +41,105 @@ end
 def LTSd (ag : agent) s l s' := @next_agent_state_from_dlabel ag.state_type (ag.loop s) l = s'
 
 end loc
+
+open temporal
+
+def sys_dlabel_to_local {agents : map ip agent}
+ (ag : agents.member) (s : @system_state agents) : 
+  sys_dlabel s → option (dlabel (ag.value.loop (s.local_state ag)))
+| (sys_dlabel.mk ag' aupdate) := do
+  plift.up H ← precondition (ag' = ag),
+  some (eq.rec_on H aupdate)
+
+universes u
+
+lemma precondition_true {P : Prop} {A : Type u} [decP : decidable P]
+  {f : plift P → option A}
+  (H : P)
+  : option_bind (precondition P) f = f (plift.up H)
+:= begin
+unfold precondition,
+induction decP; dsimp [precondition],
+{ contradiction },
+{ simp [option_bind],
+}
+end
+
+lemma precondition_false {P : Prop} [decP : decidable P]
+  (H : ¬ P)
+  : precondition P = none
+:= begin
+unfold precondition,
+induction decP; dsimp [precondition],
+{ simp [option_bind], },
+{ contradiction
+}
+end
+
+lemma precondition_true_bind {P : Prop} {A : Type} [decP : decidable P]
+  {f : plift P → option A}
+  (H : P)
+  : precondition P >>= f = f (plift.up H)
+:= precondition_true H
+
+lemma next_state_local 
+  (agents : map ip agent)
+  (ag : mapd.member agents)
+  (incoming : incoming_items)
+  (a_next : act ag.value.state_type)
+  (label : dlabel a_next)
+  (new_state : (ag.value).state_type)
+  (updatef : global_state_t → global_state_t)
+  (Hx1 : next_agent_state_from_dlabel (ag.key) (ag.value) incoming label = some (new_state, updatef))
+: loc.next_agent_state_from_dlabel label = new_state
+:= begin
+induction label, dsimp [loc.next_agent_state_from_dlabel, dlabel.cont_result],
+dsimp [next_agent_state_from_dlabel] at Hx1,
+apply_in Hx1 option_bind_some,
+induction Hx1 with updatef H,
+induction H with H1 H2,
+dsimp [next_agent_state_from_dlabel] at H2,
+generalize Hx : cont r = x, rw Hx at H2,
+clear Hx, induction x, dsimp,
+dsimp [next_agent_state_from_dlabel] at H2,
+injection H2 with H, clear H2, injection H with H1 H2
+end
+
+theorem refines
+  (agents : map ip agent)
+  (ag : agents.member)
+ : Refinement (@LTSd agents) (SkipLTS (loc.LTSd ag.value))
+:= { S_refine := λ s, s.local_state ag
+   , L_refine := sys_dlabel_to_local ag
+   , refines := begin
+   intros s l s' H,
+   unfold LTSd at H, induction l,
+   simp only [next_state_from_dlabel] at H,
+   simp only [sys_dlabel_to_local],
+   rename ag_1 ag',
+   apply_in H option_bind_some,
+   induction H with Hx Hx', induction Hx' with Hx1 Hx2,
+   induction Hx with new_state updatef,
+   dsimp [next_state_from_dlabel] at Hx2,
+   injection Hx2 with Hx2', clear Hx2,
+   subst s', dsimp,
+   apply (if Hag : ag' = ag then _ else _),
+   { -- I go! 
+     rw (precondition_true_bind Hag),
+     dsimp [sys_dlabel_to_local], induction Hag,
+     dsimp, unfold SkipLTS,
+     unfold loc.LTSd,
+     rw lookup_update_refl,
+     generalize Hls : (ag'.value).loop (s.local_state ag') = ls,
+     rw Hls at label, rename label label',
+     apply next_state_local, assumption,
+   },
+   { --Someone else goes
+   rw (precondition_false Hag),
+   dsimp [has_bind.bind, option_bind],
+   dsimp [SkipLTS],
+   rw (lookup_update_different Hag),
+   },
+   end
+   }
 end network
